library/init/data/nat/basic.lean
@@ -58,40 +58,157 @@ def {u} repeat {α : Type u} (f : ℕ → α → α) : ℕ → α → α
 instance : inhabited ℕ :=
 ⟨nat.zero⟩
 
-@[simp] lemma nat_zero_eq_zero : nat.zero = 0 :=
+protected def pow (b : ℕ) : ℕ → ℕ
+| 0        := 1
+| (succ n) := pow n * b
+
+instance : has_pow nat nat :=
+⟨nat.pow⟩
+
+/- nat.add theorems -/
+
+protected theorem zero_add : ∀ n : ℕ, 0 + n = n
+| 0     := rfl
+| (n+1) := congr_arg succ (zero_add n)
+
+theorem succ_add : ∀ n m : ℕ, (succ n) + m = succ (n + m)
+| n 0     := rfl
+| n (m+1) := congr_arg succ (succ_add n m)
+
+theorem add_succ (n m : ℕ) : n + succ m = succ (n + m) :=
 rfl
 
-/- properties of inequality -/
+protected theorem add_zero (n : ℕ) : n + 0 = n :=
+rfl
+
+theorem add_one (n : ℕ) : n + 1 = succ n :=
+rfl
+
+theorem succ_eq_add_one (n : ℕ) : succ n = n + 1 :=
+rfl
+
+protected theorem add_comm : ∀ n m : ℕ, n + m = m + n
+| n 0     := eq.symm (nat.zero_add n)
+| n (m+1) :=
+  suffices succ (n + m) = succ (m + n), from
+    eq.symm (succ_add m n) ▸ this,
+  congr_arg succ (add_comm n m)
+
+protected theorem add_assoc : ∀ n m k : ℕ, (n + m) + k = n + (m + k)
+| n m 0        := rfl
+| n m (succ k) := congr_arg succ (add_assoc n m k)
+
+protected theorem add_left_comm : ∀ (n m k : ℕ), n + (m + k) = m + (n + k) :=
+left_comm nat.add nat.add_comm nat.add_assoc
+
+protected theorem add_right_comm : ∀ (n m k : ℕ), (n + m) + k = (n + k) + m :=
+right_comm nat.add nat.add_comm nat.add_assoc
+
+protected theorem add_left_cancel : ∀ {n m k : ℕ}, n + m = n + k → m = k
+| 0        m k h := nat.zero_add m ▸ nat.zero_add k ▸ h
+| (succ n) m k h :=
+  have n+m = n+k, from
+    have succ (n + m) = succ (n + k), from succ_add n m ▸ succ_add n k ▸ h,
+    nat.no_confusion this id,
+  add_left_cancel this
+
+protected theorem add_right_cancel {n m k : ℕ} (h : n + m = k + m) : n = k :=
+have m + n = m + k, from nat.add_comm n m ▸ nat.add_comm k m ▸ h,
+nat.add_left_cancel this
+
+/- nat.mul theorems -/
+
+protected theorem mul_zero (n : ℕ) : n * 0 = 0 :=
+rfl
+
+theorem mul_succ (n m : ℕ) : n * succ m = n * m + n :=
+rfl
+
+protected theorem zero_mul : ∀ (n : ℕ), 0 * n = 0
+| 0        := rfl
+| (succ n) := (mul_succ 0 n).symm ▸ (zero_mul n).symm ▸ rfl
+
+theorem succ_mul : ∀ (n m : ℕ), (succ n) * m = (n * m) + m
+| n 0        := rfl
+| n (succ m) :=
+  have succ (n * m + m + n) = succ (n * m + n + m), from
+    congr_arg succ (nat.add_right_comm _ _ _),
+  (mul_succ n m).symm ▸ (mul_succ (succ n) m).symm ▸ (succ_mul n m).symm ▸ this
+
+protected theorem mul_comm : ∀ (n m : ℕ), n * m = m * n
+| n 0        := (nat.zero_mul n).symm ▸ (nat.mul_zero n).symm ▸ rfl
+| n (succ m) := (mul_succ n m).symm ▸ (succ_mul m n).symm ▸ (mul_comm n m).symm ▸ rfl
+
+protected theorem mul_one : ∀ (n : ℕ), n * 1 = n :=
+nat.zero_add
+
+protected theorem one_mul (n : ℕ) : 1 * n = n :=
+nat.mul_comm n 1 ▸ nat.mul_one n
+
+protected theorem left_distrib : ∀ (n m k : ℕ), n * (m + k) = n * m + n * k
+| 0        m k := (nat.zero_mul (m + k)).symm ▸ (nat.zero_mul m).symm ▸ (nat.zero_mul k).symm ▸ rfl
+| (succ n) m k := calc
+  succ n * (m + k)
+        = n * (m + k) + (m + k)      : succ_mul _ _
+    ... = (n * m + n * k) + (m + k)  : left_distrib n m k ▸ rfl
+    ... = n * m + (n * k + (m + k))  : nat.add_assoc _ _ _
+    ... = n * m + (m + (n * k + k))  : congr_arg (λ x, n*m + x) (nat.add_left_comm _ _ _)
+    ... = (n * m + m) + (n * k + k)  : (nat.add_assoc _ _ _).symm
+    ... = (n * m + m) + succ n * k   : succ_mul n k ▸ rfl
+    ... = succ n * m + succ n * k    : succ_mul n m ▸ rfl
+
+protected theorem right_distrib (n m k : ℕ) : (n + m) * k = n * k + m * k :=
+calc (n + m) * k
+       = k * (n + m)   : nat.mul_comm _ _
+  ...  = k * n + k * m : nat.left_distrib _ _ _
+  ...  = n * k + k * m : nat.mul_comm n k ▸ rfl
+  ...  = n * k + m * k : nat.mul_comm m k ▸ rfl
+
+protected theorem mul_assoc : ∀ (n m k : ℕ), (n * m) * k = n * (m * k)
+| n m 0        := rfl
+| n m (succ k) := calc
+  n * m * succ k
+       = n * m * (k + 1)           : rfl
+   ... = (n * m * k) + n * m * 1   : nat.left_distrib _ _ _
+   ... = (n * m * k) + n * m       : (nat.mul_one (n*m)).symm ▸ rfl
+   ... = (n * (m * k)) + n * m     : (mul_assoc n m k).symm ▸ rfl
+   ... = n * (m * k + m)           : (nat.left_distrib n (m*k) m).symm
+   ... = n * (m * succ k)          : nat.mul_succ m k ▸ rfl
+
+/- Inequalities -/
 
 @[refl] protected def le_refl : ∀ a : ℕ, a ≤ a :=
 less_than_or_equal.refl
 
-lemma le_succ (n : ℕ) : n ≤ succ n :=
+theorem le_succ (n : ℕ) : n ≤ succ n :=
 less_than_or_equal.step (nat.le_refl n)
 
-lemma succ_le_succ {n m : ℕ} : n ≤ m → succ n ≤ succ m :=
+theorem succ_le_succ {n m : ℕ} : n ≤ m → succ n ≤ succ m :=
 λ h, less_than_or_equal.rec (nat.le_refl (succ n)) (λ a b, less_than_or_equal.step) h
 
-lemma zero_le : ∀ (n : ℕ), 0 ≤ n
+theorem succ_lt_succ {a b : ℕ} : a < b → succ a < succ b :=
+succ_le_succ
+
+theorem zero_le : ∀ (n : ℕ), 0 ≤ n
 | 0     := nat.le_refl 0
 | (n+1) := less_than_or_equal.step (zero_le n)
 
-lemma zero_lt_succ (n : ℕ) : 0 < succ n :=
+theorem zero_lt_succ (n : ℕ) : 0 < succ n :=
 succ_le_succ (zero_le n)
 
 def succ_pos := zero_lt_succ
 
-lemma not_succ_le_zero : ∀ (n : ℕ), succ n ≤ 0 → false
+theorem not_succ_le_zero : ∀ (n : ℕ), succ n ≤ 0 → false
 .
 
-lemma not_lt_zero (a : ℕ) : ¬ a < 0 := not_succ_le_zero a
+theorem not_lt_zero (a : ℕ) : ¬ a < 0 := not_succ_le_zero a
 
-lemma pred_le_pred {n m : ℕ} : n ≤ m → pred n ≤ pred m :=
+theorem pred_le_pred {n m : ℕ} : n ≤ m → pred n ≤ pred m :=
 λ h, less_than_or_equal.rec_on h
   (nat.le_refl (pred n))
   (λ n, nat.rec (λ a b, b) (λ a b c, less_than_or_equal.step) n)
 
-lemma le_of_succ_le_succ {n m : ℕ} : succ n ≤ succ m → n ≤ m :=
+theorem le_of_succ_le_succ {n m : ℕ} : succ n ≤ succ m → n ≤ m :=
 pred_le_pred
 
 instance decidable_le : ∀ a b : ℕ, decidable (a ≤ b)
@@ -106,38 +223,41 @@ instance decidable_le : ∀ a b : ℕ, decidable (a ≤ b)
 instance decidable_lt : ∀ a b : ℕ, decidable (a < b) :=
 λ a b, nat.decidable_le (succ a) b
 
-protected lemma eq_or_lt_of_le {a b : ℕ} (h : a ≤ b) : a = b ∨ a < b :=
+protected theorem eq_or_lt_of_le {a b : ℕ} (h : a ≤ b) : a = b ∨ a < b :=
 less_than_or_equal.cases_on h (or.inl rfl) (λ n h, or.inr (succ_le_succ h))
 
-lemma lt_succ_of_le {a b : ℕ} : a ≤ b → a < succ b :=
+theorem lt_succ_of_le {a b : ℕ} : a ≤ b → a < succ b :=
 succ_le_succ
 
-@[simp] lemma succ_sub_succ_eq_sub (a b : ℕ) : succ a - succ b = a - b :=
+protected theorem sub_zero (n : ℕ) : n - 0 = n :=
+rfl
+
+theorem succ_sub_succ_eq_sub (a b : ℕ) : succ a - succ b = a - b :=
 nat.rec_on b
   (show succ a - succ zero = a - zero, from (eq.refl (succ a - succ zero)))
   (λ b, congr_arg pred)
 
-lemma not_succ_le_self : ∀ n : ℕ, ¬succ n ≤ n :=
+theorem not_succ_le_self : ∀ n : ℕ, ¬succ n ≤ n :=
 λ n, nat.rec (not_succ_le_zero 0) (λ a b c, b (le_of_succ_le_succ c)) n
 
-protected lemma lt_irrefl (n : ℕ) : ¬n < n :=
+protected theorem lt_irrefl (n : ℕ) : ¬n < n :=
 not_succ_le_self n
 
-protected lemma le_trans {n m k : ℕ} (h1 : n ≤ m) : m ≤ k → n ≤ k :=
+protected theorem le_trans {n m k : ℕ} (h1 : n ≤ m) : m ≤ k → n ≤ k :=
 less_than_or_equal.rec h1 (λ p h2, less_than_or_equal.step)
 
-lemma pred_le : ∀ (n : ℕ), pred n ≤ n
+theorem pred_le : ∀ (n : ℕ), pred n ≤ n
 | 0        := less_than_or_equal.refl 0
 | (succ a) := less_than_or_equal.step (less_than_or_equal.refl a)
 
-lemma pred_lt : ∀ {n : ℕ}, n ≠ 0 → pred n < n
+theorem pred_lt : ∀ {n : ℕ}, n ≠ 0 → pred n < n
 | 0        h := absurd rfl h
 | (succ a) h := lt_succ_of_le (less_than_or_equal.refl _)
 
-lemma sub_le (a b : ℕ) : a - b ≤ a :=
+theorem sub_le (a b : ℕ) : a - b ≤ a :=
 nat.rec_on b (nat.le_refl (a - 0)) (λ b₁, nat.le_trans (pred_le (a - b₁)))
 
-lemma sub_lt : ∀ {a b : ℕ}, 0 < a → 0 < b → a - b < a
+theorem sub_lt : ∀ {a b : ℕ}, 0 < a → 0 < b → a - b < a
 | 0     b     h1 h2 := absurd h1 (nat.lt_irrefl 0)
 | (a+1) 0     h1 h2 := absurd h2 (nat.lt_irrefl 0)
 | (a+1) (b+1) h1 h2 :=
@@ -145,67 +265,295 @@ lemma sub_lt : ∀ {a b : ℕ}, 0 < a → 0 < b → a - b < a
     show a - b < succ a, from
     lt_succ_of_le (sub_le a b)
 
-protected lemma lt_of_lt_of_le {n m k : ℕ} : n < m → m ≤ k → n < k :=
+protected theorem lt_of_lt_of_le {n m k : ℕ} : n < m → m ≤ k → n < k :=
 nat.le_trans
 
-/- Basic nat.add lemmas -/
-protected lemma zero_add : ∀ n : ℕ, 0 + n = n
-| 0     := rfl
-| (n+1) := congr_arg succ (zero_add n)
+protected theorem le_of_eq {n m : ℕ} (p : n = m) : n ≤ m :=
+p ▸ less_than_or_equal.refl n
 
-lemma succ_add : ∀ n m : ℕ, (succ n) + m = succ (n + m)
-| n 0     := rfl
-| n (m+1) := congr_arg succ (succ_add n m)
+theorem le_succ_of_le {n m : ℕ} (h : n ≤ m) : n ≤ succ m :=
+nat.le_trans h (le_succ m)
 
-lemma add_succ (n m : ℕ) : n + succ m = succ (n + m) :=
+theorem le_of_succ_le {n m : ℕ} (h : succ n ≤ m) : n ≤ m :=
+nat.le_trans (le_succ n) h
+
+protected theorem le_of_lt {n m : ℕ} (h : n < m) : n ≤ m :=
+le_of_succ_le h
+
+def lt.step {n m : ℕ} : n < m → n < succ m := less_than_or_equal.step
+
+theorem eq_zero_or_pos : ∀ (n : ℕ), n = 0 ∨ n > 0
+| 0     := or.inl rfl
+| (n+1) := or.inr (succ_pos _)
+
+protected theorem lt_trans {n m k : ℕ} (h₁ : n < m) : m < k → n < k :=
+nat.le_trans (less_than_or_equal.step h₁)
+
+protected theorem lt_of_le_of_lt {n m k : ℕ} (h₁ : n ≤ m) : m < k → n < k :=
+nat.le_trans (succ_le_succ h₁)
+
+def lt.base (n : ℕ) : n < succ n := nat.le_refl (succ n)
+
+theorem lt_succ_self (n : ℕ) : n < succ n := lt.base n
+
+protected theorem le_antisymm {n m : ℕ} (h₁ : n ≤ m) : m ≤ n → n = m :=
+less_than_or_equal.cases_on h₁ (λ a, rfl) (λ a b c, absurd (nat.lt_of_le_of_lt b c) (nat.lt_irrefl n))
+
+protected theorem lt_or_ge : ∀ (a b : ℕ), a < b ∨ a ≥ b
+| a 0     := or.inr (zero_le a)
+| a (b+1) :=
+  match lt_or_ge a b with
+  | or.inl h := or.inl (le_succ_of_le h)
+  | or.inr h :=
+    match nat.eq_or_lt_of_le h with
+    | or.inl h1 := or.inl (h1 ▸ lt_succ_self b)
+    | or.inr h1 := or.inr h1
+    end
+  end
+
+protected theorem le_total (m n : ℕ) : m ≤ n ∨ n ≤ m :=
+or.imp_left nat.le_of_lt (nat.lt_or_ge m n)
+
+protected theorem lt_of_le_and_ne {m n : ℕ} (h1 : m ≤ n) : m ≠ n → m < n :=
+or.resolve_right (or.swap (nat.eq_or_lt_of_le h1))
+
+theorem eq_zero_of_le_zero {n : nat} (h : n ≤ 0) : n = 0 :=
+nat.le_antisymm h (zero_le _)
+
+theorem lt_of_succ_lt {a b : ℕ} : succ a < b → a < b :=
+le_of_succ_le
+
+theorem lt_of_succ_lt_succ {a b : ℕ} : succ a < succ b → a < b :=
+le_of_succ_le_succ
+
+theorem lt_of_succ_le {a b : ℕ} (h : succ a ≤ b) : a < b := h
+
+theorem succ_le_of_lt {a b : ℕ} (h : a < b) : succ a ≤ b := h
+
+theorem le_add_right : ∀ (n k : ℕ), n ≤ n + k
+| n 0     := nat.le_refl n
+| n (k+1) := le_succ_of_le (le_add_right n k)
+
+theorem le_add_left (n m : ℕ): n ≤ m + n :=
+nat.add_comm n m ▸ le_add_right n m
+
+theorem le.dest : ∀ {n m : ℕ}, n ≤ m → ∃ k, n + k = m
+| n ._ (less_than_or_equal.refl ._)  := ⟨0, rfl⟩
+| n ._ (@less_than_or_equal.step ._ m h) :=
+  match le.dest h with
+  | ⟨w, hw⟩ := ⟨succ w, hw ▸ add_succ n w⟩
+  end
+
+theorem le.intro {n m k : ℕ} (h : n + k = m) : n ≤ m :=
+h ▸ le_add_right n k
+
+protected theorem not_le_of_gt {a b : nat} (h : a > b) : ¬ a ≤ b :=
+λ (h₁ : a ≤ b),
+  or.elim (nat.lt_or_ge a b)
+  (λ h₂, absurd (nat.lt_trans h h₂) (nat.lt_irrefl _))
+  (λ h₂, have heq : a = b, from nat.le_antisymm h₁ h₂, absurd (@eq.subst _ _ _ _ heq h) (nat.lt_irrefl b))
+
+theorem gt_of_not_le {a b : nat} (h : ¬ a ≤ b) : a > b :=
+or.elim (nat.lt_or_ge b a)
+  (λ h₁, h₁)
+  (λ h₁, absurd h₁ h)
+
+protected theorem lt_of_le_of_ne {a b : nat} (h₁ : a ≤ b) (h₂ : a ≠ b) : a < b :=
+or.elim (nat.lt_or_ge a b)
+  (λ h₃, h₃)
+  (λ h₃, absurd (nat.le_antisymm h₁ h₃) h₂)
+
+protected theorem add_le_add_left {n m : ℕ} (h : n ≤ m) (k : ℕ) : k + n ≤ k + m :=
+match le.dest h with
+| ⟨w, hw⟩ :=
+  have k + n + w = k + m, from
+    calc k + n + w = k + (n + w) : nat.add_assoc _ _ _
+            ...    = k + m       : congr_arg _ hw,
+  le.intro this
+end
+
+protected theorem add_le_add_right {n m : ℕ} (h : n ≤ m) (k : ℕ) : n + k ≤ m + k :=
+calc
+  n + k = k + n : nat.add_comm _ _
+    ... ≤ k + m : nat.add_le_add_left h k
+    ... = m + k : nat.add_comm _ _
+
+protected theorem add_lt_add_left {n m : ℕ} (h : n < m) (k : ℕ) : k + n < k + m :=
+lt_of_succ_le (add_succ k n ▸ nat.add_le_add_left (succ_le_of_lt h) k)
+
+protected theorem add_lt_add_right {n m : ℕ} (h : n < m) (k : ℕ) : n + k < m + k :=
+nat.add_comm k m ▸ nat.add_comm k n ▸ nat.add_lt_add_left h k
+
+protected theorem zero_lt_one : 0 < (1:nat) :=
+zero_lt_succ 0
+
+theorem le_of_lt_succ {m n : nat} : m < succ n → m ≤ n :=
+le_of_succ_le_succ
+
+lemma add_le_add {a b c d : nat} (h₁ : a ≤ b) (h₂ : c ≤ d) : a + c ≤ b + d :=
+nat.le_trans (nat.add_le_add_right h₁ c) (nat.add_le_add_left h₂ b)
+
+lemma add_lt_add {a b c d : nat} (h₁ : a < b) (h₂ : c < d) : a + c < b + d :=
+nat.lt_trans (nat.add_lt_add_right h₁ c) (nat.add_lt_add_left h₂ b)
+
+/- Basic theorems for comparing numerals -/
+
+theorem nat_zero_eq_zero : nat.zero = 0 :=
 rfl
 
-protected lemma add_zero (n : ℕ) : n + 0 = n :=
-rfl
+protected theorem one_ne_zero : 1 ≠ (0 : ℕ) :=
+assume h, nat.no_confusion h
 
-lemma add_one (n : ℕ) : n + 1 = succ n :=
-rfl
+protected theorem zero_ne_one : 0 ≠ (1 : ℕ) :=
+assume h, nat.no_confusion h
 
-lemma succ_eq_add_one (n : ℕ) : succ n = n + 1 :=
-rfl
+theorem succ_ne_zero (n : ℕ) : succ n ≠ 0 :=
+assume h, nat.no_confusion h
 
-/- Basic lemmas for comparing numerals -/
-
-protected lemma bit0_succ_eq (n : ℕ) : bit0 (succ n) = succ (succ (bit0 n)) :=
+protected theorem bit0_succ_eq (n : ℕ) : bit0 (succ n) = succ (succ (bit0 n)) :=
 show succ (succ n + n) = succ (succ (n + n)), from
 congr_arg succ (succ_add n n)
 
-protected lemma zero_lt_bit0 : ∀ {n : nat}, n ≠ 0 → 0 < bit0 n
+protected theorem zero_lt_bit0 : ∀ {n : nat}, n ≠ 0 → 0 < bit0 n
 | 0        h := absurd rfl h
 | (succ n) h :=
   calc 0 < succ (succ (bit0 n)) : zero_lt_succ _
      ... = bit0 (succ n)        : (nat.bit0_succ_eq n).symm
 
-protected lemma zero_lt_bit1 (n : nat) : 0 < bit1 n :=
+protected theorem zero_lt_bit1 (n : nat) : 0 < bit1 n :=
 zero_lt_succ _
 
-protected lemma bit0_ne_zero : ∀ {n : ℕ}, n ≠ 0 → bit0 n ≠ 0
+protected theorem bit0_ne_zero : ∀ {n : ℕ}, n ≠ 0 → bit0 n ≠ 0
 | 0     h := absurd rfl h
 | (n+1) h :=
   suffices (n+1) + (n+1) ≠ 0, from this,
   suffices succ ((n+1) + n) ≠ 0, from this,
   λ h, nat.no_confusion h
 
-protected lemma bit1_ne_zero (n : ℕ) : bit1 n ≠ 0 :=
+protected theorem bit1_ne_zero (n : ℕ) : bit1 n ≠ 0 :=
 show succ (n + n) ≠ 0, from
 λ h, nat.no_confusion h
 
-/- Exponentiation -/
+protected theorem bit1_eq_succ_bit0 (n : ℕ) : bit1 n = succ (bit0 n) :=
+rfl
 
-protected def pow (b : ℕ) : ℕ → ℕ
-| 0        := 1
-| (succ n) := pow n * b
+protected theorem bit1_succ_eq (n : ℕ) : bit1 (succ n) = succ (succ (bit1 n)) :=
+eq.trans (nat.bit1_eq_succ_bit0 (succ n)) (congr_arg succ (nat.bit0_succ_eq n))
 
-instance : has_pow nat nat :=
-⟨nat.pow⟩
+protected theorem bit1_ne_one : ∀ {n : ℕ}, n ≠ 0 → bit1 n ≠ 1
+| 0     h h1 := absurd rfl h
+| (n+1) h h1 := nat.no_confusion h1 (λ h2, absurd h2 (succ_ne_zero _))
 
-lemma pow_succ (b n : ℕ) : b^(succ n) = b^n * b := rfl
+protected theorem bit0_ne_one : ∀ n : ℕ, bit0 n ≠ 1
+| 0     h := absurd h (ne.symm nat.one_ne_zero)
+| (n+1) h :=
+  have h1 : succ (succ (n + n)) = 1, from succ_add n n ▸ h,
+  nat.no_confusion h1
+    (λ h2, absurd h2 (succ_ne_zero (n + n)))
 
-@[simp] lemma pow_zero (b : ℕ) : b^0 = 1 := rfl
+protected theorem add_self_ne_one : ∀ (n : ℕ), n + n ≠ 1
+| 0     h := nat.no_confusion h
+| (n+1) h :=
+  have h1 : succ (succ (n + n)) = 1, from succ_add n n ▸ h,
+  nat.no_confusion h1 (λ h2, absurd h2 (nat.succ_ne_zero (n + n)))
+
+protected theorem bit1_ne_bit0 : ∀ (n m : ℕ), bit1 n ≠ bit0 m
+| 0     m     h := absurd h (ne.symm (nat.add_self_ne_one m))
+| (n+1) 0     h :=
+  have h1 : succ (bit0 (succ n)) = 0, from h,
+  absurd h1 (nat.succ_ne_zero _)
+| (n+1) (m+1) h :=
+  have h1 : succ (succ (bit1 n)) = succ (succ (bit0 m)), from
+    nat.bit0_succ_eq m ▸ nat.bit1_succ_eq n ▸ h,
+  have h2 : bit1 n = bit0 m, from
+    nat.no_confusion h1 (λ h2', nat.no_confusion h2' (λ h2'', h2'')),
+  absurd h2 (bit1_ne_bit0 n m)
+
+protected theorem bit0_ne_bit1 : ∀ (n m : ℕ), bit0 n ≠ bit1 m :=
+λ n m : nat, ne.symm (nat.bit1_ne_bit0 m n)
+
+protected theorem bit0_inj : ∀ {n m : ℕ}, bit0 n = bit0 m → n = m
+| 0     0     h := rfl
+| 0     (m+1) h := absurd h.symm (succ_ne_zero _)
+| (n+1) 0     h := absurd h (succ_ne_zero _)
+| (n+1) (m+1) h :=
+  have (n+1) + n = (m+1) + m, from nat.no_confusion h id,
+  have n + (n+1) = m + (m+1), from nat.add_comm (m+1) m ▸ nat.add_comm (n+1) n ▸ this,
+  have succ (n + n) = succ (m + m), from this,
+  have n + n = m + m, from nat.no_confusion this id,
+  have n = m, from bit0_inj this,
+  congr_arg (+1) this
+
+protected theorem bit1_inj : ∀ {n m : ℕ}, bit1 n = bit1 m → n = m :=
+λ n m h,
+have succ (bit0 n) = succ (bit0 m), from nat.bit1_eq_succ_bit0 n ▸ nat.bit1_eq_succ_bit0 m ▸ h,
+have bit0 n = bit0 m, from nat.no_confusion this id,
+nat.bit0_inj this
+
+protected theorem bit0_ne {n m : ℕ} : n ≠ m → bit0 n ≠ bit0 m :=
+λ h₁ h₂, absurd (nat.bit0_inj h₂) h₁
+
+protected theorem bit1_ne {n m : ℕ} : n ≠ m → bit1 n ≠ bit1 m :=
+λ h₁ h₂, absurd (nat.bit1_inj h₂) h₁
+
+protected theorem zero_ne_bit0 {n : ℕ} : n ≠ 0 → 0 ≠ bit0 n :=
+λ h, ne.symm (nat.bit0_ne_zero h)
+
+protected theorem zero_ne_bit1 (n : ℕ) : 0 ≠ bit1 n :=
+ne.symm (nat.bit1_ne_zero n)
+
+protected theorem one_ne_bit0 (n : ℕ) : 1 ≠ bit0 n :=
+ne.symm (nat.bit0_ne_one n)
+
+protected theorem one_ne_bit1 {n : ℕ} : n ≠ 0 → 1 ≠ bit1 n :=
+λ h, ne.symm (nat.bit1_ne_one h)
+
+protected theorem one_lt_bit1 : ∀ {n : nat}, n ≠ 0 → 1 < bit1 n
+| 0        h := absurd rfl h
+| (succ n) h :=
+  suffices succ 0 < succ (succ (bit1 n)), from
+    (nat.bit1_succ_eq n).symm ▸ this,
+  succ_lt_succ (zero_lt_succ _)
+
+protected theorem one_lt_bit0 : ∀ {n : nat}, n ≠ 0 → 1 < bit0 n
+| 0        h := absurd rfl h
+| (succ n) h :=
+  suffices succ 0 < succ (succ (bit0 n)), from
+    (nat.bit0_succ_eq n).symm ▸ this,
+  succ_lt_succ (zero_lt_succ _)
+
+protected lemma bit0_lt {n m : nat} (h : n < m) : bit0 n < bit0 m :=
+nat.add_lt_add h h
+
+protected lemma bit1_lt {n m : nat} (h : n < m) : bit1 n < bit1 m :=
+succ_lt_succ (nat.add_lt_add h h)
+
+protected lemma bit0_lt_bit1 {n m : nat} (h : n ≤ m) : bit0 n < bit1 m :=
+lt_succ_of_le (nat.add_le_add h h)
+
+protected lemma bit1_lt_bit0 : ∀ {n m : nat}, n < m → bit1 n < bit0 m
+| n 0        h := absurd h (not_lt_zero _)
+| n (succ m) h :=
+  have n ≤ m, from le_of_lt_succ h,
+  have succ (n + n) ≤ succ (m + m),      from succ_le_succ (add_le_add this this),
+  have succ (n + n) ≤ succ m + m,        from (succ_add m m).symm ▸ this,
+  show succ (n + n) < succ (succ m + m), from lt_succ_of_le this
+
+protected lemma one_le_bit1 (n : ℕ) : 1 ≤ bit1 n :=
+show 1 ≤ succ (bit0 n), from
+succ_le_succ (zero_le (bit0 n))
+
+protected lemma one_le_bit0 : ∀ (n : ℕ), n ≠ 0 → 1 ≤ bit0 n
+| 0     h := absurd rfl h
+| (n+1) h :=
+  suffices 1 ≤ succ (succ (bit0 n)), from
+    eq.symm (nat.bit0_succ_eq n) ▸ this,
+  succ_le_succ (zero_le (succ (bit0 n)))
+
+/- power -/
+
+theorem pow_succ (b n : ℕ) : b^(succ n) = b^n * b := rfl
+
+theorem pow_zero (b : ℕ) : b^0 = 1 := rfl
 
 end nat
