library/init/data/basic.lean
@@ -9,5 +9,5 @@ import init.data.nat.basic init.data.prod init.data.sum.basic
 import init.data.sigma.basic init.data.subtype.basic
 import init.data.fin.basic init.data.list.basic init.data.char.basic
 import init.data.string.basic init.data.option.basic init.data.set
-import init.data.unsigned.basic init.data.ordering.basic init.data.repr
+import init.data.uint init.data.ordering.basic init.data.repr
 import init.data.to_string
