library/init/data/char/lemmas.lean
@@ -1,5 +1,5 @@
 prelude
-import init.meta init.logic init.data.nat.lemmas
+import init.meta init.logic init.data.nat.basic
 import init.data.char.basic
 
 namespace char
