library/init/data/fin/default.lean
@@ -4,4 +4,4 @@ Released under Apache 2.0 license as described in the file LICENSE.
 Author: Leonardo de Moura
 -/
 prelude
-import init.data.fin.basic init.data.fin.ops
+import init.data.fin.basic
