library/init/data/nat/div.lean
@@ -18,8 +18,27 @@ protected def div := well_founded.fix lt_wf div.F
 instance : has_div nat :=
 ⟨nat.div⟩
 
-lemma div_def_aux (x y : nat) : x / y = if h : 0 < y ∧ y ≤ x then (x - y) / y + 1 else 0 :=
+private lemma div_def_aux (x y : nat) : x / y = if h : 0 < y ∧ y ≤ x then (x - y) / y + 1 else 0 :=
 congr_fun (well_founded.fix_eq lt_wf div.F x) y
+
+lemma div_def (x y : nat) : x / y = if 0 < y ∧ y ≤ x then (x - y) / y + 1 else 0 :=
+dif_eq_if (0 < y ∧ y ≤ x) ((x - y) / y + 1) 0 ▸ div_def_aux x y
+
+private lemma {u} div.induction.F
+        (C : nat → nat → Sort u)
+        (h₁ : ∀ x y, 0 < y ∧ y ≤ x → C (x - y) y → C x y)
+        (h₂ : ∀ x y, ¬(0 < y ∧ y ≤ x) → C x y)
+        (x : nat) (f : ∀ (x₁ : nat), x₁ < x → ∀ (y : nat), C x₁ y) (y : nat) : C x y :=
+if h : 0 < y ∧ y ≤ x then h₁ x y h (f (x - y) (div_rec_lemma h) y) else h₂ x y h
+
+@[elab_as_eliminator]
+lemma {u} div.induction_on
+      {C : nat → nat → Sort u}
+      (x y : nat)
+      (h₁ : ∀ x y, 0 < y ∧ y ≤ x → C (x - y) y → C x y)
+      (h₂ : ∀ x y, ¬(0 < y ∧ y ≤ x) → C x y)
+      : C x y :=
+well_founded.fix nat.lt_wf (div.induction.F C h₁ h₂) x y
 
 private def mod.F (x : nat) (f : Π x₁, x₁ < x → nat → nat) (y : nat) : nat :=
 if h : 0 < y ∧ y ≤ x then f (x - y) (div_rec_lemma h) y else x
@@ -29,7 +48,49 @@ protected def mod := well_founded.fix lt_wf mod.F
 instance : has_mod nat :=
 ⟨nat.mod⟩
 
-lemma mod_def_aux (x y : nat) : x % y = if h : 0 < y ∧ y ≤ x then (x - y) % y else x :=
+private lemma mod_def_aux (x y : nat) : x % y = if h : 0 < y ∧ y ≤ x then (x - y) % y else x :=
 congr_fun (well_founded.fix_eq lt_wf mod.F x) y
+
+lemma mod_def (x y : nat) : x % y = if 0 < y ∧ y ≤ x then (x - y) % y else x :=
+dif_eq_if (0 < y ∧ y ≤ x) ((x - y) % y) x ▸ mod_def_aux x y
+
+@[elab_as_eliminator]
+lemma {u} mod.induction_on
+      {C : nat → nat → Sort u}
+      (x y : nat)
+      (h₁ : ∀ x y, 0 < y ∧ y ≤ x → C (x - y) y → C x y)
+      (h₂ : ∀ x y, ¬(0 < y ∧ y ≤ x) → C x y)
+      : C x y :=
+div.induction_on x y h₁ h₂
+
+lemma mod_zero (a : nat) : a % 0 = a :=
+suffices (if 0 < 0 ∧ 0 ≤ a then (a - 0) % 0 else a) = a, from (mod_def a 0).symm ▸ this,
+have h : ¬ (0 < 0 ∧ 0 ≤ a), from λ ⟨h₁, _⟩, absurd h₁ (nat.lt_irrefl _),
+if_neg h
+
+lemma mod_eq_of_lt {a b : nat} (h : a < b) : a % b = a :=
+suffices (if 0 < b ∧ b ≤ a then (a - b) % b else a) = a, from (mod_def a b).symm ▸ this,
+have h' : ¬(0 < b ∧ b ≤ a), from λ ⟨_, h₁⟩, absurd h₁ (nat.not_le_of_gt h),
+if_neg h'
+
+lemma mod_eq_sub_mod {a b : nat} (h : a ≥ b) : a % b = (a - b) % b :=
+or.elim (eq_zero_or_pos b)
+  (λ h₁, h₁.symm ▸ (nat.sub_zero a).symm ▸ rfl)
+  (λ h₁, (mod_def a b).symm ▸ if_pos ⟨h₁, h⟩)
+
+lemma mod_lt (x : nat) {y : nat} : y > 0 → x % y < y :=
+mod.induction_on x y
+  (λ x y ⟨_, h₁⟩ h₂ h₃,
+   have ih  : (x - y) % y < y, from h₂ h₃,
+   have heq : x % y = (x - y) % y, from mod_eq_sub_mod h₁,
+   heq.symm ▸ ih)
+  (λ x y h₁ h₂,
+    have h₁ : ¬ 0 < y ∨ ¬ y ≤ x, from iff.mp (decidable.not_and_iff_or_not _ _) h₁,
+    or.elim h₁
+     (λ h₁, absurd h₂ h₁)
+     (λ h₁,
+        have hgt : y > x, from gt_of_not_le h₁,
+        have heq : x % y = x, from mod_eq_of_lt hgt,
+        heq.symm ▸ hgt))
 
 end nat
