library/init/data/uint.lean
@@ -1,0 +1,54 @@
+/-
+Copyright (c) 2018 Microsoft Corporation. All rights reserved.
+Released under Apache 2.0 license as described in the file LICENSE.
+Authors: Leonardo de Moura
+-/
+prelude
+import init.data.fin.basic
+
+open nat
+def uint32_sz : nat := 4294967296
+def uint32 := fin uint32_sz
+
+def uint64_sz : nat := 18446744073709551616
+def uint64 := fin uint64_sz
+
+instance : decidable_eq uint32 :=
+have decidable_eq (fin uint32_sz), from fin.decidable_eq _,
+this
+
+instance : decidable_eq uint64 :=
+have decidable_eq (fin uint64_sz), from fin.decidable_eq _,
+this
+
+instance : has_zero uint32 := ⟨fin.of_nat 0⟩
+instance : has_one uint32  := ⟨fin.of_nat 1⟩
+instance : has_add uint32  := ⟨fin.add⟩
+instance : has_sub uint32  := ⟨fin.sub⟩
+instance : has_mul uint32  := ⟨fin.mul⟩
+instance : has_mod uint32  := ⟨fin.mod⟩
+instance : has_div uint32  := ⟨fin.div⟩
+instance : has_lt uint32   := ⟨fin.lt⟩
+instance : has_le uint32   := ⟨fin.le⟩
+
+instance : has_zero uint64 := ⟨fin.of_nat 0⟩
+instance : has_one uint64  := ⟨fin.of_nat 1⟩
+instance : has_add uint64  := ⟨fin.add⟩
+instance : has_sub uint64  := ⟨fin.sub⟩
+instance : has_mul uint64  := ⟨fin.mul⟩
+instance : has_mod uint64  := ⟨fin.mod⟩
+instance : has_div uint64  := ⟨fin.div⟩
+instance : has_lt uint64   := ⟨fin.lt⟩
+instance : has_le uint64   := ⟨fin.le⟩
+
+def uint32.of_nat (n : nat) : uint32 :=
+fin.of_nat n
+
+def uint32.to_nat (u : uint32) : nat :=
+fin.val u
+
+def uint64.of_nat (n : nat) : uint64 :=
+fin.of_nat n
+
+def uint64.to_nat (u : uint64) : nat :=
+fin.val u
