library/init/meta/name.lean
@@ -10,7 +10,7 @@ import init.data.ordering.basic init.coe init.data.to_string
 inductive name
 | anonymous  : name
 | mk_string  : string → name → name
-| mk_numeral : unsigned → name → name
+| mk_numeral : uint32 → name → name
 
 /-- Gadget for automatic parameter support. This is similar to the opt_param gadget, but it uses
     the tactic declaration names tac_name to synthesize the argument.
@@ -29,7 +29,7 @@ def mk_str_name (n : name) (s : string) : name :=
 name.mk_string s n
 
 def mk_num_name (n : name) (v : nat) : name :=
-name.mk_numeral (unsigned.of_nat' v) n
+name.mk_numeral (uint32.of_nat v) n
 
 def mk_simple_name (s : string) : name :=
 mk_str_name name.anonymous s
