library/init/meta/well_founded_tactics.lean
@@ -4,7 +4,7 @@ Released under Apache 2.0 license as described in the file LICENSE.
 Authors: Leonardo de Moura
 -/
 prelude
-import init.meta init.data.sigma.lex init.data.nat.lemmas init.data.list.instances
+import init.meta init.data.sigma.lex init.data.list.instances
 import init.data.string.instances
 
 /-- Argument for using_well_founded
